Compiler/Skeletons/mkMap.v
@@ -1,29 +1,80 @@
 Require Import LibTactics Psatz.
-Require Import GPUCSL scan_lib CSLTactics.
+Require Import GPUCSL SkelLib scan_lib CSLTactics.
 Require Import CUDALib TypedTerm.
-Require Import CSLLemma CodeGen CUDALib Correctness CSLTactics.
+Require Import Skel_lemma CSLLemma CodeGen CUDALib Correctness CSLTactics.
 Require Import Host.
+
+Open Scope string_scope.
 
 Section mkMap.
 
 Variable ntrd nblk : nat.
 
 Variable GA : list Skel.Typ.
-Variable dom cod : Skel.Typ.
-Variable arr : var -> (cmd * vars dom).
-Variable func : vars dom -> (cmd * vars cod).
+Variable avar_env : AVarEnv GA.
+Variable aptr_env : APtrEnv GA.
+Variable aeval_env : AEvalEnv GA.
+Hypothesis Haok : aenv_ok avar_env.
 
-Definition out : vars cod := maptys fst (out_name cod).
-Definition len : vars Skel.TZ := out_len_name.
+Variable dom cod : Skel.Typ.
+Variable arr : Skel.AE GA dom.
+Variable arr_c : var -> (cmd * vars dom).
+Hypothesis arr_ok : ae_ok avar_env arr arr_c.
+
+Variable f : Skel.Func GA (Skel.Fun1 dom cod).
+Variable f_c : vars dom -> (cmd * vars cod).
+Hypothesis f_ok : func_ok avar_env f f_c.
+
+Variable result : Skel.aTypDenote cod.
+Hypothesis eval_map_ok :
+  Skel.skelDenote _ _ (Skel.Map _ _ _ f arr) aeval_env = Some result.
+
+Lemma eval_arr_ok :
+  { arr_res | Skel.aeDenote _ _ arr aeval_env = Some arr_res}.
+Proof.
+  simpl in *; unfold Monad.bind_opt in *.
+  destruct Skel.aeDenote; simpl in *; inverts eval_map_ok; eexists; eauto.
+Qed.
+
+Definition arr_res : Skel.aTypDenote dom := let (a, _) := eval_arr_ok in a.
+
+Definition eval_arr_ok' : Skel.aeDenote _ _ arr aeval_env = Some arr_res.
+Proof.
+  unfold arr_res; destruct eval_arr_ok; eauto.
+Qed.
+
+Lemma eval_f_ok : 
+  { f_res | forall i, i < length arr_res ->
+                      Skel.funcDenote _ _ f aeval_env (gets' arr_res i) = Some (f_res i)}.
+Proof.
+  simpl in *; unfold Monad.bind_opt in *.
+  lets H: eval_arr_ok'; generalize arr_res H; intros arr_res H'; clear H.
+  rewrite H' in eval_map_ok.
+  exists (fun i : nat => nth i result (defval')).
+  intros i Hi.
+  forwards*: (>>mapM_some i (@defval' dom) (@defval' cod)).
+  destruct lt_dec; eauto; lia.
+Qed.
+
+Definition f_res := let (f, _) := eval_f_ok in f.
+Lemma eval_f_ok' : forall i, i < length arr_res -> Skel.funcDenote _ _ f aeval_env (gets' arr_res i) = Some (f_res i).
+Proof.
+  unfold f_res; destruct eval_f_ok; simpl; eauto.
+Qed.
+
+Definition outArr ty := locals "_arrOut" ty 0.
+
+Notation out := (outArr cod).
+Notation len := out_len_name.
 Definition t := locals "t" dom 0.
 
 Definition mkMap_cmd inv :=
   "i" :T Int ::= "tid" +C "bid" *C Zn ntrd ;;
   WhileI inv ("i" <C len) (
-    fst (arr "i") ;;
-    assigns t (ty2ctys dom) (v2e (snd (arr "i"))) ;;
-    fst (func t) ;;
-    writes (v2gl out +os "i") (v2e (snd (func t))) ;;
+    fst (arr_c "i") ;;
+    assigns t (ty2ctys dom) (v2e (snd (arr_c "i"))) ;;
+    fst (f_c t) ;;
+    writes (v2gl out +os "i") (v2e (snd (f_c t))) ;;
     "i" ::= Zn ntrd *C Zn nblk +C "i"
   )%exp.
 
@@ -32,16 +83,73 @@ Definition mkMap : kernel :=
   let params_in := flatten_avars arr_vars in
   let params_out := (out_len_name, Int) :: flatTup (out_name cod) in
   {| params_of := params_out ++ params_in;
-     body_of := Pr nil (mkMap_cmd FalseP) |}.
+     body_of := GCSL.Pr nil (mkMap_cmd FalseP) |}.
 
-Variable avar_env : AVarEnv GA.
-Variable aptr_env : APtrEnv GA.
-Variable aeval_env : AEvalEnv GA.
+Notation RP n := (1 / injZ (Zn n))%Qc.
+Notation p := (RP (nblk * ntrd)).
 
-Lemma mkMap_cmd_ok BS (tid : Fin.t ntrd) : 
+Variable outp : vals cod.
+Variable outs : list (vals cod).
+Hypothesis outs_length : length outs = length result.
+Definition outRes (ls : list (vals cod)) := arrays (val2gl outp) ls 1.
+Definition outEnv := out |=> outp.
+
+Section thread_ok.
+Variable tid : Fin.t ntrd.
+Variable bid : Fin.t nblk.
+
+Notation arri a := (skip a (ntrd * nblk) (nf tid + nf bid * ntrd)).
+Notation result' := (arr2CUDA result).
+
+Definition inv'  :=
+  Ex j i,
+  (kernelInv avar_env aptr_env aeval_env 
+             (arrays' (val2gl outp) (arri (firstn i result' ++ skipn i outs)) 1) 
+             (i = j * (ntrd * nblk) + (nf tid + nf bid * nblk) /\
+              i < length arr_res)
+             (len |-> Zn (length arr_res) ::
+              "i" |-> Zn i ::
+              out |=> outp) p).
+
+Ltac prove_not_local :=
+  let x := fresh "x" in
+  let H := fresh "H" in
+  simpl; intros x H;
+  des_disj H; substs;
+  unfold is_param; simpl; try congruence.
+
+Lemma remove_var_out ty ps x :
+  prefix "_" x = false
+  -> remove_var (outArr ty |=> ps) x = outArr ty |=> ps.
+Proof.
+  intros Hpref.
+  apply remove_var_disjoint; simpl.
+  unfold outArr; intros Hc.
+  apply in_map_iff in Hc as (? & ? & ?); substs.
+  destruct x0; simpl in *.
+  apply mpss_in in H0.
+  forwards* (j & Heq & ?): locals_pref; substs.
+  inverts Heq; simpl in *; congruence.
+Qed.
+
+Lemma mkMap_cmd_ok BS : 
   CSL BS tid
-      (kernelInv avar_env aptr_env aeval_env Emp True nil 1)
-      (mkMap_cmd FalseP)
-      (kernelInv avar_env aptr_env aeval_env Emp True nil 1).
+      (kernelInv avar_env aptr_env aeval_env (arrays' (val2gl outp) (arri outs) 1)
+                 True
+                 ("tid" |-> Zn (nf tid)
+                  :: "bid" |-> Zn (nf bid)
+                  :: len |-> Zn (length arr_res)
+                  :: out |=> outp) p)
+      (mkMap_cmd inv')
+      (kernelInv avar_env aptr_env aeval_env (arrays' (val2gl outp) (arri (arr2CUDA result)) 1) True nil p).
+Proof.
+  eapply rule_seq.
+  applys* kernelInv_inner.
+  prove_not_local. 
+  hoare_forward.
+  rewrite remove_var_out; eauto.
+  unfold inv'; hoare_forward.
+  hoare_forward.
 Abort.
+End thread_ok.
 End mkMap.
